prove hist_epochs_puts abstraction for relating a client's history of puts with its per-epoch knowledge of its pk. the latter provides a more intuitive top-level spec, culminating in lookup_msv'

src/program_proof/pav/client_hist.v
@@ -2,36 +2,159 @@ From Perennial.program_proof.pav Require Import prelude.
 From Goose.github_com.mit_pdos.pav Require Import kt.
 
 From Perennial.program_proof.pav Require Import
-  advrpc auditor core classes client cryptoffi
-  evidence logical_audit logical_hist merkle rpc serde server.
+  advrpc auditor core classes client cryptoffi evidence
+  logical_audit logical_hist merkle msv rpc serde server.
+
+Lemma last_replicate {A} (x : A) n :
+  last (replicate n x) = match n with 0%nat => None | S _ => Some x end.
+Proof.
+  rewrite last_lookup length_replicate.
+  destruct n; [done|].
+  rewrite lookup_replicate_2; [done|lia].
+Qed.
+
+Lemma last_replicate_option_app {A} (l : list (option A)) n :
+  mjoin $ last (l ++ replicate n (mjoin $ last l)) = mjoin $ last l.
+Proof.
+  rewrite last_app last_replicate.
+  repeat case_match; try done.
+  naive_solver.
+Qed.
+
+Lemma filter_snoc {A} (P : A → Prop) `{∀ x, Decision (P x)} l x :
+  filter P (l ++ [x]) = filter P l ++ (if decide (P x) then [x] else []).
+Proof. by rewrite filter_app. Qed.
+
+Module hist_epochs_puts.
+
+(* length-extends hist with its last element. *)
+Definition lookup_epochs_hist (hist : list $ option pk_ty) (ep : w64) :=
+  match hist !! (uint.nat ep) with
+  | Some opt_pk => opt_pk
+  | None => mjoin $ last hist
+  end.
+
+Definition lookup_puts_hist (hist : list map_val_ty) (ep : w64) :=
+  snd <$> (last $ filter (λ x, uint.Z x.1 <= uint.Z ep) hist).
+
+Definition reln epochs puts :=
+  ∀ ep,
+  lookup_epochs_hist epochs ep = lookup_puts_hist puts ep.
+
+Lemma update_replicate epochs puts n :
+  reln epochs puts →
+  reln (epochs ++ replicate n (mjoin $ last epochs)) puts.
+Proof.
+  rewrite /reln /lookup_epochs_hist.
+  intros Hreln ep.
+  ospecialize (Hreln ep).
+  rewrite last_replicate_option_app.
+  destruct (decide (uint.Z ep < Z.of_nat $ length epochs)).
+  { rewrite lookup_app_l; [done|word]. }
+  rewrite lookup_ge_None_2 in Hreln; [|word].
+  rewrite lookup_app_r; [|word].
+  case_match; [|done].
+  apply lookup_replicate in H.
+  intuition.
+  by simplify_eq/=.
+Qed.
+
+Lemma update_new epochs puts ep pk :
+  (* something to tie together epochs and puts (ep). *)
+  Z.of_nat $ length epochs = uint.Z ep →
+  reln epochs puts →
+  reln (epochs ++ [Some pk]) (puts ++ [(ep, pk)]).
+Proof.
+  rewrite /reln /lookup_epochs_hist /lookup_puts_hist.
+  intros ? Hreln ep0.
+  rewrite filter_snoc /=.
+  destruct (decide (uint.Z ep0 < Z.of_nat $ length epochs)).
+  (* revert lookups back to the original hists. *)
+  - ospecialize (Hreln ep0).
+    (* epochs. *)
+    rewrite lookup_app_l; [|word].
+    opose proof (list_lookup_lt epochs (uint.nat ep0) _) as [? Ht]; [word|].
+    rewrite Ht in Hreln |-*.
+    (* puts. *)
+    case_decide; [word|].
+    by list_simplifier.
+  (* extract snoc'd entry out of hists. *)
+  - clear Hreln.
+    (* puts. *)
+    case_decide; [|word].
+    rewrite !last_snoc /=.
+    (* epochs. *)
+    rewrite lookup_app_r; [|word].
+    case_match; [|done].
+    by list_simplifier.
+Qed.
+
+End hist_epochs_puts.
 
 Module ClientHist.
 Record t :=
   mk {
     γ: gname;
     uid: w64;
-    (* pks differs from the client struct.
-    it tracks all our actual keys. *)
-    pks: list map_val_ty;
+    (* epochs_hist allows stating the "intuitive" KT consistency property:
+    that a client knows its key at every epoch. *)
+    epochs_hist: list (option pk_ty);
+    (* puts_hist tracks all our puts.
+    it needs to be visible to connect to the physical puts_hist. *)
+    puts_hist: list map_val_ty;
     next_epoch: w64;
-    (* hist_epoch differs from the client struct.
-    it's epoch validity for the history, which only gets updated by
-    Put and SelfMon, not Get. *)
-    hist_epoch: w64;
     serv: Server.t;
     serv_is_good: bool;
   }.
 Global Instance eta : Settable _ :=
-  settable! mk <γ; uid; pks; next_epoch; hist_epoch; serv; serv_is_good>.
+  settable! mk <γ; uid; epochs_hist; puts_hist; next_epoch; serv; serv_is_good>.
 
 Section defs.
 Context `{!heapGS Σ, !pavG Σ}.
 
 Definition own (ptr : loc) (obj : t) : iProp Σ :=
-  "%Hlt_ep" ∷ ⌜ uint.Z obj.(hist_epoch) <= uint.Z obj.(next_epoch) ⌝ ∗
-  "Hcli" ∷ Client.own ptr (Client.mk obj.(γ) obj.(uid) (W64 $ length obj.(pks))
-    obj.(next_epoch) obj.(serv) obj.(serv_is_good)) ∗
-  "#Hhist" ∷ is_hist obj.(γ) obj.(serv).(Server.vrf_pk) obj.(uid) obj.(pks) obj.(hist_epoch).
+  "%Hlt_ep" ∷ ⌜ Z.of_nat $ length obj.(epochs_hist) <= uint.Z obj.(next_epoch) ⌝ ∗
+  "%Hhist_reln" ∷ ⌜ hist_epochs_puts.reln obj.(epochs_hist) obj.(puts_hist) ⌝ ∗
+
+  "Hcli" ∷ Client.own ptr (Client.mk obj.(γ) obj.(uid)
+    (W64 $ length obj.(puts_hist)) obj.(next_epoch) obj.(serv)
+    obj.(serv_is_good)) ∗
+  "#Hhist" ∷ is_hist obj.(γ) obj.(serv).(Server.vrf_pk) obj.(uid)
+    obj.(puts_hist) (W64 $ length obj.(epochs_hist)).
+
+Lemma lookup_msv' ptr_c c ep opt_pk γaudit aud_ep :
+  c.(epochs_hist) !! (uint.nat ep) = Some opt_pk →
+  uint.Z ep < uint.Z aud_ep →
+  own ptr_c c -∗
+  logical_audit_post c.(γ) γaudit c.(serv).(Server.vrf_pk) aud_ep -∗
+  ∃ opt_mapval,
+  ⌜ snd <$> opt_mapval = opt_pk ⌝ ∗
+  msv γaudit c.(serv).(Server.vrf_pk) ep c.(uid) opt_mapval.
+Proof.
+  iIntros (Hlook ?) "H #Haudit". iNamed "H".
+  iDestruct (hist_to_msv ep with "Hhist Haudit") as "H".
+  { apply lookup_lt_Some in Hlook. word. }
+  { (* this requires knowing that for any epochs hist idx,
+    can make a puts hist, valid for idx, that relates to it. *)
+Abort.
+
+Lemma lookup_msv ptr_c c ep opt_pk γaudit aud_ep :
+  c.(epochs_hist) !! (uint.nat ep) = Some opt_pk →
+  Z.of_nat $ length c.(epochs_hist) <= uint.Z aud_ep →
+  own ptr_c c -∗
+  logical_audit_post c.(γ) γaudit c.(serv).(Server.vrf_pk) aud_ep -∗
+  ∃ opt_mapval,
+  ⌜ snd <$> opt_mapval = opt_pk ⌝ ∗
+  msv γaudit c.(serv).(Server.vrf_pk) ep c.(uid) opt_mapval.
+Proof.
+  iIntros (Hlook ?) "H #Haudit". iNamed "H".
+  iDestruct (hist_to_msv ep with "Hhist Haudit") as "$".
+  { apply lookup_lt_Some in Hlook. word. }
+  { word. }
+  iPureIntro.
+  ospecialize (Hhist_reln ep).
+  by rewrite /hist_epochs_puts.lookup_epochs_hist Hlook in Hhist_reln.
+Qed.
 
 End defs.
 End ClientHist.
@@ -50,13 +173,17 @@ Lemma wp_ClientHist__Put ptr_c c sl_pk d0 (pk : list w8) :
     "Hsl_pk" ∷ own_slice_small sl_pk byteT d0 pk ∗
     "Hown_err" ∷ ClientErr.own ptr_err err c.(ClientHist.serv).(Server.sig_pk) ∗
     "%Hgenie" ∷ ⌜ c.(ClientHist.serv_is_good) = true → err.(ClientErr.Err) = false ⌝ ∗
+
     "Herr" ∷ (if err.(ClientErr.Err)
       then
         "Hcli" ∷ ClientHist.own ptr_c c
       else
-        let new_c := set ClientHist.pks (λ x, (x ++ [(ep, pk)]))
-          (set ClientHist.next_epoch (λ _, word.add ep (W64 1))
-          (set ClientHist.hist_epoch (λ _, word.add ep (W64 1)) c)) in
+        let new_c :=
+          set ClientHist.next_epoch (λ _, word.add ep (W64 1))
+          (set ClientHist.epochs_hist (λ x, x ++
+            replicate (uint.nat ep - length x) (mjoin $ last x) ++
+            [Some pk])
+          (set ClientHist.puts_hist (λ x, x ++ [(ep, pk)]) c)) in
         "Hcli" ∷ ClientHist.own ptr_c new_c)
   }}}.
 Proof.
@@ -66,12 +193,20 @@ Proof.
   simpl. iIntros "*". iNamed 1.
   iApply "HΦ". iFrame "∗%".
   case_match; iNamed "Herr"; [by iFrame "∗#"|].
-  iSplit; simpl in *; [done|]; iSplit.
-  - rewrite length_app. simpl.
+  do 3 try iSplit; simpl in *.
+  - rewrite !length_app length_replicate /=. word.
+  - iPureIntro.
+    rewrite (assoc (++)).
+    apply hist_epochs_puts.update_new.
+    { rewrite length_app length_replicate. word. }
+    by apply hist_epochs_puts.update_replicate.
+  - rewrite length_app /=.
     replace (W64 (_ + _)%nat) with
-      (word.add (W64 $ length pks) (W64 1)); [|word].
+      (word.add (W64 $ length puts_hist) (W64 1)); [|word].
     iFrame.
-  - iApply hist_extend_put; [..|iFrame "#"]; try word.
+  - rewrite !length_app length_replicate /=.
+    iEval (replace (W64 _) with (word.add ep (W64 1)) by word).
+    iApply (hist_extend_put with "[$Hhist $His_put_post]"); word.
 Qed.
 
 Lemma wp_ClientHist__SelfMon ptr_c c :
@@ -88,8 +223,10 @@ Lemma wp_ClientHist__SelfMon ptr_c c :
       then
         "Hcli" ∷ ClientHist.own ptr_c c
       else
-        let new_c := set ClientHist.next_epoch (λ _, word.add ep (W64 1))
-          (set ClientHist.hist_epoch (λ _, word.add ep (W64 1)) c) in
+        let new_c :=
+          set ClientHist.next_epoch (λ _, word.add ep (W64 1))
+          (set ClientHist.epochs_hist (λ x, x ++
+            replicate (uint.nat ep + 1 - length x) (mjoin $ last x)) c) in
         "Hcli" ∷ ClientHist.own ptr_c new_c)
   }}}.
 Proof.
@@ -98,38 +235,15 @@ Proof.
   wp_apply (wp_Client__SelfMon with "[$Hcli]").
   simpl. iIntros "*". iNamed 1.
   iApply "HΦ". iFrame "∗%".
-  case_match; iNamed "Herr"; iFrame "∗#"; simpl; [done|].
-  iSplit; [done|].
-  (* TODO: maybe iApply bug. this doesn't work.
-  iApply (hist_extend_selfmon with "[# $]"). *)
-  iApply hist_extend_selfmon; [..|iFrame "#"]; word.
-Qed.
-
-Lemma wp_ClientHist__Get ptr_c c (uid : w64) :
-  {{{
-    "Hcli" ∷ ClientHist.own ptr_c c
-  }}}
-  Client__Get #ptr_c #uid
-  {{{
-    err sl_pk (is_reg : bool) (ep : w64) ptr_err,
-    RET (#is_reg, slice_val sl_pk, #ep, #ptr_err);
-    "Hown_err" ∷ ClientErr.own ptr_err err c.(ClientHist.serv).(Server.sig_pk) ∗
-    "%Hgenie" ∷ ⌜ c.(ClientHist.serv_is_good) = true → err.(ClientErr.Err) = false ⌝ ∗
-
-    "Herr" ∷ (if err.(ClientErr.Err)
-      then
-        "Hcli" ∷ ClientHist.own ptr_c c
-      else
-        let new_c := set ClientHist.next_epoch (λ _, word.add ep (W64 1)) c in
-        "Hcli" ∷ ClientHist.own ptr_c new_c)
-  }}}.
-Proof.
-  iIntros (Φ) "H HΦ". iNamed "H". iNamed "Hcli".
-  destruct c. simpl in *.
-  wp_apply (wp_Client__Get with "[$Hcli]").
-  simpl. iIntros "*". iNamed 1.
-  iApply "HΦ". iFrame "∗%".
-  case_match; iNamed "Herr"; iFrame "∗#"; simpl; [done|word].
+  case_match; iNamed "Herr"; [by iFrame "∗#"|].
+  do 3 try iSplit; simpl in *.
+  - rewrite !length_app length_replicate. word.
+  - iPureIntro.
+    by apply hist_epochs_puts.update_replicate.
+  - iFrame.
+  - rewrite !length_app length_replicate.
+    iEval (replace (W64 _) with (word.add ep (W64 1)) by word).
+    iApply (hist_extend_selfmon with "[$Hhist $His_selfmon_post]"); word.
 Qed.
 
 End proof.
